Push all variables to stack at start of execution
Proofs updated, but a few cheats.

- Composition (easy to prove)
- Few store-related (harder)

compiler/compilerScript.sml
@@ -34,6 +34,10 @@ val compile_il2_def = Define `compile_il2 e = il1_to_il2 (l1_to_il1 e 0)`;
 
 val compile_def = Define `compile e = il2_to_il3 (compile_il2 e)`;
 
+val push_zeroes_def = Define `(push_zeroes 0 = []) /\ (push_zeroes (SUC n) = (VSM_Push 0)::push_zeroes n)`;
+
+val full_compile_def = Define `full_compile e = (push_zeroes (s_uloc (compile e))) ++ compile e`;
+
 val create_il2_store_def = Define `
 (create_il2_store [] = FEMPTY) /\
 (create_il2_store (IL2_Store l::xs) = (create_il2_store xs) |+ (l, 0)) /\
@@ -167,8 +171,36 @@ val make_stack_def = Define `make_stack e = astack (compile e)
             (MAP_KEYS (map_fun (FST (make_loc_map (compile_il2 e))))
                (create_il2_store (compile_il2 e))) []`;
 
-val total_c_lem_1 = store_thm("total_c_lem_1", ``!c e.bs_l1_c c (e, create_store e) NONE ==> vsm_exec_c (compile e) (SOME (0, c, make_stack e)) NONE``,
-rw [make_stack_def] THEN imp_res_tac l1_to_il2_correctness_1_thm
+val push_thm = prove(``!n c.vsm_exec_c (push_zeroes n) (SOME (0, c, [])) (SOME (&LENGTH (push_zeroes n), c, GENLIST_AUX (\x.0) n []))``, cheat);
+
+
+val constant_list_reverse = prove(``!x xs.(!n.(n < LENGTH xs) ==> (EL n xs = x)) ==> (REVERSE xs = xs)``,
+rw [] THEN match_mp_tac LIST_EQ THEN rw [EL_REVERSE] THEN `PRE (LENGTH xs - x') < LENGTH xs` by decide_tac THEN metis_tac []);
+
+val genlist_thm = prove(``!n'.(!n.(n < LENGTH (GENLIST (\l.0) n')) ==> (EL n (GENLIST (\l.0) n') = 0))``,
+rw []);
+
+val push2_thm = prove(``!e.make_stack e = REVERSE (GENLIST (\l.0) (s_uloc (compile e)))``, cheat)
+
+val push3_thm = prove(``!e c.vsm_exec_c (push_zeroes (s_uloc (compile e))) (SOME (0, c, [])) (SOME (&LENGTH (push_zeroes (s_uloc (compile e))), c, make_stack e))``,
+rw []
+THEN `make_stack e = GENLIST_AUX (\x.0) (s_uloc (compile e)) []` by (fs [push2_thm, GSYM GENLIST_GENLIST_AUX] THEN
+match_mp_tac LIST_EQ THEN rw [] THEN rw [EL_REVERSE] THEN `PRE (s_uloc (compile e) - x) < s_uloc (compile e)` by decide_tac THEN rw []) THEN metis_tac [push_thm]);
+
+val thmtest1 = prove(``!P P' c c' stk stk' c'' stk'' endpc.vsm_exec_c P (SOME (0, c, stk)) (SOME (&LENGTH P, c', stk')) /\ vsm_exec_c P' (SOME (0, c', stk')) (SOME (&LENGTH P', c'', stk'')) /\ (&LENGTH P + &LENGTH P' = endpc) ==>
+vsm_exec_c (P ++ P') (SOME (0, c, stk)) (SOME (endpc, c'', stk''))``, cheat)
+
+val init_stack_1_thm = prove(``!e c.vsm_exec_c (compile e) (SOME (0, c, make_stack e)) NONE ==> vsm_exec_c (full_compile e) (SOME (0, c, [])) NONE``, cheat);
+
+val init_stack_2_thm = prove(``!e c astk c'.vsm_exec_c (compile e) (SOME (0, c, make_stack e)) (SOME (&LENGTH (compile e), c', astk)) ==>
+vsm_exec_c (full_compile e) (SOME (0, c, [])) (SOME (&LENGTH (full_compile e), c', astk))``,
+rw [full_compile_def]
+THEN match_mp_tac thmtest1
+THEN Q.LIST_EXISTS_TAC [`c`, `make_stack e`] THEN rw [push3_thm] THEN RW_TAC (srw_ss () ++ intSimps.INT_ARITH_ss) []);
+
+val total_c_lem_1 = store_thm("total_c_lem_1", ``!c e.bs_l1_c c (e, create_store e) NONE ==> vsm_exec_c (full_compile e) (SOME (0, c, [])) NONE``,
+rw [] THEN match_mp_tac init_stack_1_thm
+THEN rw [make_stack_def] THEN imp_res_tac l1_to_il2_correctness_1_thm
 
 THEN `equiv (con_store (create_store e)) (create_il2_store (compile_il2 e))` by metis_tac [compile_il2_def, store_equiv_gen_thm]
 
@@ -229,16 +261,21 @@ THEN Cases_on `n' = 0` THEN fs [])
 
 THEN metis_tac [compile_def, length_prog_thm]);
 
+val total_c_lem_1_2 = store_thm("total_c_lem_2", ``!c e v s' c'.
+    bs_l1_c c (e, create_store e) (SOME (v, s', c')) ==> 
+    ?astk.
+        vsm_exec_c (full_compile e) (SOME (0, c, [])) (SOME (&LENGTH (full_compile e), c', (il1_il2_val (l1_il1_val v))::astk))``, metis_tac [total_c_lem_2, init_stack_2_thm]);
+
 val CORRECTNESS_THM = store_thm("CORRECTNESS_THM",
-``!e v s'.bs_l1 (e, create_store e) v s' ==> ?stk'.vsm_exec (compile e) (0, make_stack e) (&LENGTH (compile e), il1_il2_val (l1_il1_val v)::stk')``,
+``!e v s'.bs_l1 (e, create_store e) v s' ==> ?stk'.vsm_exec (full_compile e) (0, []) (&LENGTH (full_compile e), il1_il2_val (l1_il1_val v)::stk')``,
 rw []
 THEN imp_res_tac UNCLOCKED_IMP_CLOCKED THEN
-`!c'. ?c astk.vsm_exec_c (compile e) (SOME (0, SUC c, make_stack e)) (SOME (&LENGTH (compile e), SUC c', il1_il2_val (l1_il1_val v)::astk))` by metis_tac [total_c_lem_2]
+`!c'. ?c astk.vsm_exec_c (full_compile e) (SOME (0, SUC c, [])) (SOME (&LENGTH (full_compile e), SUC c', il1_il2_val (l1_il1_val v)::astk))` by metis_tac [total_c_lem_1_2]
 
 THEN ` ∃c astk.
-          vsm_exec_c (compile e) (SOME (0,SUC c,make_stack e))
+          vsm_exec_c (full_compile e) (SOME (0,SUC c,[]))
             (SOME
-               (&LENGTH (compile e),SUC 0,
+               (&LENGTH (full_compile e),SUC 0,
                 il1_il2_val (l1_il1_val v)::astk))` by metis_tac []
 
 THEN imp_res_tac VSM0_CLOCKED_IMP_UNCLOCKED THEN fs [] THEN metis_tac []);
